Major update of verify.strm/na_strm

nola/examples/logic/verify/na_strm.v
@@ -1,94 +1,103 @@
 (** * Verification on non-atomic shared mutable singly linked streams *)
 
-From nola.examples.logic Require Export na_inv.
+From nola.examples.logic Require Export na_inv verify.strm_base.
 From nola.iris Require Export wp.
 From nola.examples.heap_lang Require Export proofmode notation.
 
 (** Stream whose elements satisfy the condition [Φ] *)
-Definition na_strm {κ Γᵘ Γᵍ} (p : na_inv_pool_name) (N : namespace)
+Definition na_strm {κ Γᵘ Γᵍ} (p : na_inv_pool_name) (N N' : namespace)
   (Φ : loc → nPropL (;ᵞ Γᵘ ++ Γᵍ)) : loc → nProp κ (Γᵘ;ᵞ Γᵍ) :=
-  (rec:ˢ l, n_na_inv' (_::_) 0 p N
-    (¢ᵍ Φ l ∗ ∃ l' : loc, (l +ₗ 1) ↦ # l' ∗ %ᵍˢ 0@ l'))%n.
+  (rec:ˢ l, n_na_inv' (_::_) 0 p N (¢ᵍ Φ l) ∗
+    n_na_inv' (_::_) 0 p N' (∃ l' : loc, (l +ₗ 1) ↦ # l' ∗ %ᵍˢ 0@ l'))%n.
 
 (** Substitution over [na_strm] *)
-Fact na_strm_nsubst {κ p N V Φ Ψ l} :
-  na_strm (κ:=κ) (Γᵘ:=[V]) p N Φ l /: Ψ =
-    na_strm (Γᵘ:=[]) p N (λ l, Φ l /:ᵍ Ψ) l.
+Fact na_strm_nsubst {κ p N N' V Φ Ψ l} :
+  na_strm (κ:=κ) (Γᵘ:=[V]) p N N' Φ l /: Ψ =
+    na_strm (Γᵘ:=[]) p N N' (λ l, Φ l /:ᵍ Ψ) l.
 Proof. done. Qed.
 
 (** Interpreted [strm] *)
-Definition na_strmi `{!nintpGS Σ} s p N Φ l : iProp Σ :=
-  na_nninv s 0 p N (Φ l ∗ ∃ l' : loc, (l +ₗ 1) ↦ # l' ∗ na_strm p N Φ l').
+Definition na_strmi `{!nintpGS Σ} s p N N' Φ l : iProp Σ :=
+  na_nninv s 0 p N (Φ l) ∗ na_nninv s 0 p N'
+    (∃ l' : loc, (l +ₗ 1) ↦ # l' ∗ na_strm (Γᵘ:=[]) p N N' Φ l').
 Notation na_strmis := (na_strmi nsintp).
-
-(** Calls [f] on the first [c] elements of the stream by [d] *)
-Definition iter : val :=
-  rec: "self" "f" "c" "l" :=
-    if: "c" = #0 then #() else "f" "l";; "self" "f" ("c" - #1) (! ("l" +ₗ #1)).
-
-(** Calls [iter] with a non-deterministic [c] *)
-Definition iter_nd : val := λ: "f" "l", iter "f" Ndnat "l".
 
 Section verify.
   Context `{!nintpGS Σ}.
 
   (** [na_strm] is interpreted into [na_strmi] *)
-  Fact na_strm_strmi {κ p N Φ l s} :
-    ⟦ na_strm p N Φ l ⟧{κ}(s) ⊣⊢ na_strmi s p N Φ l.
+  Fact na_strm_strmi {κ p N N' Φ l s} :
+    ⟦ na_strm p N N' Φ l ⟧{κ}(s) ⊣⊢ na_strmi s p N N' Φ l.
   Proof. by rewrite/= rew_eq_hwf /=. Qed.
 
   (** Convert the predicate of [na_strmi] *)
-  Lemma na_strmi_convert `{!nsintpy Σ ih s} {p N Φ Ψ l} :
+  Lemma na_strmi_convert `{!nsintpy Σ ih s} {p N N' Φ Ψ l} :
     □ ⸨ ∀ l, (Φ l ={∅}=∗ Ψ l) ∗ (Ψ l ={∅}=∗ Φ l) ⸩(s, 0) -∗
-    na_strmi s p N Φ l -∗ na_strmi s p N Ψ l.
+    na_strmi s p N N' Φ l -∗ na_strmi s p N N' Ψ l.
   Proof.
     move: s nsintpy0 Φ Ψ l. apply (sintpy_acc (λ _, ∀ Φ Ψ l, _ -∗ _)).
-    move=> s ? Φ Ψ l. iIntros "#sΦ↔Ψ". iApply na_nninv_convert. iModIntro.
-    iApply sintpy_byintp=>/=.
-    iIntros (s' sys' [IH _]) "#to #tos' _ (Φ & %l' & ↦ & inv)".
-    rewrite rew_eq_hwf /=. iDestruct "inv" as "#inv".
-    iDestruct ("to" with "sΦ↔Ψ") as "/=Φ↔Ψ".
-    iDestruct ("tos'" with "sΦ↔Ψ") as "s'Φ↔Ψ".
-    iDestruct ("Φ↔Ψ" $! _) as "[ΦΨ ΨΦ]". iMod ("ΦΨ" with "Φ") as "$". iModIntro.
-    iSplitL "↦". { iExists _. iFrame "↦". rewrite rew_eq_hwf /=.
-      iApply (IH with "[//] inv"). }
-    iIntros "(Ψ & %l'' & ↦ & inv')". iMod ("ΨΦ" with "Ψ") as "$". iModIntro.
-    iExists _. iFrame "↦". rewrite !rew_eq_hwf /=. iDestruct "inv'" as "#inv'".
-    iApply (IH with "[]"); [|done]. iModIntro.
-    iApply (sintpy_map (sintpy0:=sys') with "[] s'Φ↔Ψ")=>/=. iClear "#".
-    iIntros (? _ _) "Φ↔Ψ %". iApply bi.sep_comm. iApply "Φ↔Ψ".
+    move=> s ? Φ Ψ l. iIntros "#sΦ↔Ψ #[??]".
+    iSplit; iApply na_nninv_convert=>//; iModIntro.
+    { iApply sintpy_map; [|done]=>/=. iIntros (s' sys' _) "Φ↔Ψ Φ".
+      iDestruct ("Φ↔Ψ" $! _) as "[ΦΨ ΨΦ]". iMod ("ΦΨ" with "Φ") as "$".
+      iIntros "!> Ψ". by iApply "ΨΦ". }
+    iApply sintpy_byintp=>/=. iIntros (s' sys' [IH _]) "_ #to _ (%l' & ↦ & st)".
+    iModIntro. rewrite rew_eq_hwf /=. iDestruct "st" as "#st".
+    iDestruct ("to" with "[//]") as "?". iSplitL.
+    { iExists _. iFrame "↦". rewrite rew_eq_hwf /=. by iApply IH. }
+    iIntros "(%l'' & ↦ & st') !>". iExists _. iFrame "↦".
+    rewrite !rew_eq_hwf /=. iApply IH; [|done]. iModIntro.
+    iApply (sintpy_map (sintpy0:=sys')); [|done]=>/=.
+    iIntros (? _ _) "Φ↔'Ψ %". iApply bi.sep_comm. iApply "Φ↔'Ψ".
   Qed.
 
-  (** [iter] terminates *)
-  Lemma twp_iter {p N Φ E F l} {f : val} {c : nat} : ↑N ⊆ E → ↑N ⊆ F →
-    na_strmis p N Φ l -∗
-    (∀ l, [[{ ⟦ Φ l ⟧ }]][nninv_wsats] f #l @ E [[{ RET #(); ⟦ Φ l ⟧ }]]) -∗
+  (** [siter] terminates under [na_strmis] *)
+  Lemma twp_siter_na {p N N' Φ E F l} {f : val} {c : nat} : ↑N' ⊆ E → ↑N' ⊆ F →
+    na_strmis p N N' Φ l -∗
+    (∀ l, [[{ na_nninvs 0 p N (Φ l) ∗ na_own p F }]][nninv_wsats]
+            f #l @ E
+          [[{ RET #(); na_own p F }]]) -∗
     [[{ na_own p F }]][nninv_wsats]
-      iter f #c #l @ E
+      siter f #c #l @ E
     [[{ RET #(); True }]].
   Proof.
-    iIntros (??) "#inv #f". iIntros (Ψ) "!> pF Ψ".
-    iInduction c as [|c] "IH" forall (l) "inv"; wp_rec; wp_pures;
+    iIntros (??) "#[ihd itl] #f". iIntros (Ψ) "!> pF Ψ".
+    iInduction c as [|c] "IH" forall (l) "ihd itl"; wp_rec; wp_pures;
       [by iApply "Ψ"|].
-    iMod (na_nninvs_acc with "inv pF")
-      as "/=((Φ & % & ↦ & inv') & pF∖N & cl)"; [done..|].
-    rewrite rew_eq_hwf /=. iDestruct "inv'" as "#inv'".
-    wp_apply ("f" with "Φ"). iIntros "Φ". wp_pures. wp_load. wp_pures.
-    iMod ("cl" with "[$Φ ↦] pF∖N") as "pF".
-    { iExists _. rewrite/= rew_eq_hwf /=. by iFrame. }
+    wp_apply ("f" with "[$pF //]"). iIntros "pF". wp_pures. wp_bind (! _)%E.
+    iMod (na_nninvs_acc with "[//] pF") as "/=((%l' & ↦ & st) & pF∖N & cl)";
+      [done..|].
+    rewrite rew_eq_hwf /=. iDestruct "st" as "#[??]". wp_load. wp_pures.
+    iMod ("cl" with "[↦] pF∖N") as "pF".
+    { iExists _. iFrame "↦". rewrite/= rew_eq_hwf /=. by iSplit. }
     have ->: (S c - 1)%Z = c by lia. by iApply ("IH" with "pF Ψ").
   Qed.
 
-  (** [iter_nd] terminates *)
-  Lemma twp_iter_nd {p N Φ E F l} {f : val} : ↑N ⊆ E → ↑N ⊆ F →
-    na_strmis p N Φ l -∗
-    (∀ l, [[{ ⟦ Φ l ⟧ }]][nninv_wsats] f #l @ E [[{ RET #(); ⟦ Φ l ⟧ }]]) -∗
+  (** [siter_nd] terminates under [na_strmis] *)
+  Lemma twp_siter_nd_na {p N N' Φ E F l} {f : val} : ↑N' ⊆ E → ↑N' ⊆ F →
+    na_strmis p N N' Φ l -∗
+    (∀ l, [[{ na_nninvs 0 p N (Φ l) ∗ na_own p F }]][nninv_wsats]
+            f #l @ E
+          [[{ RET #(); na_own p F }]]) -∗
     [[{ na_own p F }]][nninv_wsats]
-      iter_nd f #l @ E
+      siter_nd f #l @ E
     [[{ RET #(); True }]].
   Proof.
-    iIntros (??) "#? #?". iIntros (Ψ) "!> pF ?". wp_lam. wp_pures.
+    iIntros (??) "#? #?". iIntros (?) "!> pF ?". wp_lam. wp_pures.
     wp_apply twp_ndnat; [done|]. iIntros (?) "_".
-    by wp_apply (twp_iter with "[//] [] pF").
+    by wp_apply (twp_siter_na with "[] [] pF").
+  Qed.
+
+  (** Introduce a Hoare triple with [na_nninvs] *)
+  Lemma twp_na_nninvs {p N Φ E F l} {f : val} : ↑N ⊆ E → ↑N ⊆ F →
+    [[{ ⟦ Φ l ⟧ }]][nninv_wsats] f #l @ E [[{ RET #(); ⟦ Φ l ⟧ }]] -∗
+    [[{ na_nninvs 0 p N (Φ l) ∗ na_own p F }]][nninv_wsats]
+      f #l @ E
+    [[{ RET #(); na_own p F }]].
+  Proof.
+    iIntros (??) "#f". iIntros (Ψ) "!> [#? pF] Ψ". iApply twpw_fupdw_nonval=>//.
+    iMod (na_nninvs_acc with "[] pF") as "/=(Φ & pF∖N & cl)"; [done..|].
+    wp_apply ("f" with "Φ"). iIntros "Φ". iMod ("cl" with "Φ pF∖N") as "?".
+    iModIntro. by iApply "Ψ".
   Qed.
 End verify.
