nola/examples/logic/verify/strm.v
@@ -1,129 +1,169 @@
 (** * Verification on shared mutable singly linked streams *)
 
-From nola.examples.logic Require Export inv.
+From nola.examples.logic Require Export inv verify.strm_base.
 From nola.iris Require Export wp.
 From nola.examples.heap_lang Require Export proofmode notation.
 
 (** Stream whose elements satisfy the condition [Φ] *)
-Definition strm {κ Γᵘ Γᵍ} (N : namespace) (Φ : loc → nPropL (;ᵞ Γᵘ ++ Γᵍ))
+Definition strm {κ Γᵘ Γᵍ} (N N' : namespace) (Φ : loc → nPropL (;ᵞ Γᵘ ++ Γᵍ))
   : loc → nProp κ (Γᵘ;ᵞ Γᵍ) :=
-  (rec:ˢ l, n_inv' (_::_) 0 N
-    (¢ᵍ Φ l ∗ ∃ l' : loc, (l +ₗ 1) ↦ # l' ∗ %ᵍˢ 0@ l'))%n.
+  (rec:ˢ l, n_inv' (_::_) 0 N (¢ᵍ Φ l) ∗
+    n_inv' (_::_) 0 N' (∃ l' : loc, (l +ₗ 1) ↦ # l' ∗ %ᵍˢ 0@ l'))%n.
 
 (** Substitution over [strm] *)
-Fact strm_nsubst {κ N V Φ Ψ l} :
-  strm (κ:=κ) (Γᵘ:=[V]) N Φ l /: Ψ = strm (Γᵘ:=[]) N (λ l, Φ l /:ᵍ Ψ) l.
+Fact strm_nsubst {κ N N' V Φ Ψ l} :
+  strm (κ:=κ) (Γᵘ:=[V]) N N' Φ l /: Ψ = strm (Γᵘ:=[]) N N' (λ l, Φ l /:ᵍ Ψ) l.
 Proof. done. Qed.
 
 (** Interpreted [strm] *)
-Definition strmi `{!nintpGS Σ} s N Φ l : iProp Σ :=
-  nninv s 0 N (Φ l ∗ ∃ l' : loc, (l +ₗ 1) ↦ # l' ∗ strm N Φ l').
+Definition strmi `{!nintpGS Σ} s N N' Φ l : iProp Σ :=
+  nninv s 0 N (Φ l) ∗
+    nninv s 0 N' (∃ l' : loc, (l +ₗ 1) ↦ # l' ∗ strm (Γᵘ:=[]) N N' Φ l').
 Notation strmis := (strmi nsintp).
 
-(** Stream whose elements are multiples of [d] *)
-Definition mul_strmi `{!nintpGS Σ} s N (d : Z) l : iProp Σ :=
-  strmi s N (λ l, ∃ k, l ↦ #(k * d))%n l.
-Notation mul_strmis := (mul_strmi nsintp).
+(** A has_multiplier of [d] is stored at [l] *)
+Definition has_mult {κ Γ} (d : Z) l : nProp κ Γ := ∃ k, l ↦ #(k * d).
 
-(** Atomically increases the first [c] elements of the stream by [d] *)
-Definition iter_inc : val :=
-  rec: "self" "d" "c" "l" :=
+(** Increment by calling [FAA] *)
+Definition incr_faa (d : Z) : val := λ: "l", FAA "l" #d;; #().
+
+(** Posssibly increment by calling [CAS] *)
+Definition may_incr_cas' (d : Z) : val :=
+  rec: "self" "c" "l" :=
     if: "c" = #0 then #() else
-      FAA "l" "d";; "self" "d" ("c" - #1) (! ("l" +ₗ #1)).
-
-(** Calls [iter_inc] with a non-deterministic [c] *)
-Definition iter_inc_nd : val := λ: "d" "l", iter_inc "d" Ndnat "l".
-
-(** Forks [c] threads executing [iter_inc_nd] *)
-Definition iter_inc_nd_forks : val :=
-  rec: "self" "d" "c" "l" :=
-    if: "c" = #0 then #() else
-      Fork (iter_inc_nd "d" "l");; "self" "d" ("c" - #1) "l".
-
-(** Calls [iter_inc_nd_forks] with a non-deterministic [c] *)
-Definition iter_inc_nd_forks_nd : val :=
-  λ: "d" "l", iter_inc_nd_forks "d" Ndnat "l".
+      let: "n" := !"l" in
+      if: CAS "l" "n" ("n" + #d) then #() else "self" ("c" - #1) "l".
+Definition may_incr_cas (d : Z) : val :=
+  λ: "l", may_incr_cas' d Ndnat "l".
 
 Section verify.
   Context `{!nintpGS Σ}.
 
   (** [strm] is interpreted into [strmi] *)
-  Fact strm_strmi {κ N Φ l s} :
-    ⟦ strm N Φ l ⟧{κ}(s) ⊣⊢ strmi s N Φ l.
+  Fact strm_strmi {κ N N' Φ l s} :
+    ⟦ strm N N' Φ l ⟧{κ}(s) ⊣⊢ strmi s N N' Φ l.
   Proof. by rewrite/= rew_eq_hwf /=. Qed.
 
   (** Convert the predicate of [strmi] *)
-  Lemma strmi_convert `{!nsintpy Σ ih s} {N Φ Ψ l} :
+  Lemma strmi_convert `{!nsintpy Σ ih s} {N N' Φ Ψ l} :
     □ ⸨ ∀ l, (Φ l ={∅}=∗ Ψ l) ∗ (Ψ l ={∅}=∗ Φ l) ⸩(s, 0) -∗
-    strmi s N Φ l -∗ strmi s N Ψ l.
+    strmi s N N' Φ l -∗ strmi s N N' Ψ l.
   Proof.
     move: s nsintpy0 Φ Ψ l. apply (sintpy_acc (λ _, ∀ Φ Ψ l, _ -∗ _)).
-    move=> s ? Φ Ψ l. iIntros "#sΦ↔Ψ". iApply nninv_convert. iModIntro.
-    iApply sintpy_byintp=>/=.
-    iIntros (s' sys' [IH _]) "#to #tos' _ (Φ & %l' & ↦ & inv)".
-    rewrite rew_eq_hwf /=. iDestruct "inv" as "#inv".
-    iDestruct ("to" with "sΦ↔Ψ") as "/=Φ↔Ψ".
-    iDestruct ("tos'" with "sΦ↔Ψ") as "s'Φ↔Ψ".
-    iDestruct ("Φ↔Ψ" $! _) as "[ΦΨ ΨΦ]". iMod ("ΦΨ" with "Φ") as "$". iModIntro.
-    iSplitL "↦". { iExists _. iFrame "↦". rewrite rew_eq_hwf /=.
-      iApply (IH with "[//] inv"). }
-    iIntros "(Ψ & %l'' & ↦ & inv')". iMod ("ΨΦ" with "Ψ") as "$". iModIntro.
-    iExists _. iFrame "↦". rewrite !rew_eq_hwf /=. iDestruct "inv'" as "#inv'".
-    iApply (IH with "[]"); [|done]. iModIntro.
-    iApply (sintpy_map (sintpy0:=sys') with "[] s'Φ↔Ψ")=>/=. iClear "#".
-    iIntros (? _ _) "Φ↔Ψ %". iApply bi.sep_comm. iApply "Φ↔Ψ".
+    move=> s ? Φ Ψ l. iIntros "#? #[??]".
+    iSplit; iApply nninv_convert=>//; iModIntro.
+    { iApply sintpy_map; [|done]=>/=. iIntros (s' sys' _) "Φ↔Ψ Φ".
+      iDestruct ("Φ↔Ψ" $! _) as "[ΦΨ ΨΦ]". iMod ("ΦΨ" with "Φ") as "$".
+      iIntros "!> Ψ". by iApply "ΨΦ". }
+    iApply sintpy_byintp=>/=. iIntros (s' sys' [IH _]) "_ #to _ (%l' & ↦ & st)".
+    iModIntro. rewrite rew_eq_hwf /=. iDestruct "st" as "#st".
+    iDestruct ("to" with "[//]") as "?". iSplitL.
+    { iExists _. iFrame "↦". rewrite rew_eq_hwf /=. by iApply IH. }
+    iIntros "(%l'' & ↦ & st') !>". iExists _. iFrame "↦".
+    rewrite !rew_eq_hwf /=. iApply IH; [|done]. iModIntro.
+    iApply (sintpy_map (sintpy0:=sys')); [|done]=>/=.
+    iIntros (? _ _) "Φ↔'Ψ %". iApply bi.sep_comm. iApply "Φ↔'Ψ".
   Qed.
 
-  (** [iter_inc] terminates *)
-  Lemma twp_iter_inc {N E d l} {c : nat} : ↑N ⊆ E →
-    [[{ mul_strmis N d l }]][nninv_wsats]
-      iter_inc #d #c #l @ E
+  (** [siter] terminates under [strmis] *)
+  Lemma twp_siter {N N' E Φ l} {f : val} {c : nat} : ↑N' ⊆ E →
+    (∀ l : loc,
+      [[{ nninvs 0 N (Φ l) }]][nninv_wsats] f #l @ E [[{ RET #(); True }]]) -∗
+    [[{ strmis N N' Φ l }]][nninv_wsats]
+      siter f #c #l @ E
     [[{ RET #(); True }]].
   Proof.
-    iIntros (??) "#inv Φ".
-    iInduction c as [|c] "IH" forall (l) "inv"; wp_rec; wp_pures;
-      [by iApply "Φ"|].
-    wp_bind (FAA _ _). iDestruct (nninv_split with "inv") as "[ihd itl]".
-    iMod (nninvs_acc with "ihd") as "/=[[%k ↦] cl]"; [done|]. wp_faa.
-    iModIntro. iMod ("cl" with "[↦]") as "_".
-    { iExists _. have ->: ((k * d) + d = (k + 1) * d)%Z by lia. iFrame. }
-    iModIntro. wp_pures. wp_bind (! _)%E.
-    iMod (nninvs_acc with "itl") as "/=[(%& ↦ & inv') cl]"; [done|].
-    rewrite rew_eq_hwf /=. iDestruct "inv'" as "#inv'". wp_load. iModIntro.
-    iMod ("cl" with "[↦]") as "_"; [|iModIntro].
-    { iExists _. rewrite/= rew_eq_hwf /=. by iFrame. }
-    wp_pures. have ->: (S c - 1)%Z = c by lia. by iApply ("IH" with "Φ").
+    iIntros (?) "#f". iIntros (Ψ) "!> #[ihd itl] Ψ".
+    iInduction c as [|c] "IH" forall (l) "ihd itl"; wp_rec; wp_pures;
+      [by iApply "Ψ"|].
+    wp_apply "f"; [done|]. iIntros "_". wp_pures. wp_bind (! _)%E.
+    iMod (nninvs_acc with "itl") as "/=[(%l' & ↦ & st) cl]"; [done|].
+    rewrite rew_eq_hwf /=. iDestruct "st" as "#[??]". wp_load. iModIntro.
+    iMod ("cl" with "[↦]") as "_".
+    { iExists _. rewrite rew_eq_hwf /=. iFrame "↦". by iSplit. }
+    iModIntro. wp_pures. have ->: (S c - 1)%Z = c by lia.
+    by iApply ("IH" with "Ψ").
   Qed.
 
-  (** [iter_inc_nd] terminates *)
-  Lemma twp_iter_inc_nd {N E d l} : ↑N ⊆ E →
-    [[{ mul_strmis N d l }]][nninv_wsats]
-      iter_inc_nd #d #l @ E
+  (** [siter_nd] terminates under [strmis] *)
+  Lemma twp_siter_nd {N N' E Φ l} {f : val} : ↑N' ⊆ E →
+    (∀ l : loc,
+      [[{ nninvs 0 N (Φ l) }]][nninv_wsats] f #l @ E [[{ RET #(); True }]]) -∗
+    [[{ strmis N N' Φ l }]][nninv_wsats]
+      siter_nd f #l @ E
     [[{ RET #(); True }]].
   Proof.
-    iIntros (??) "#? ?". wp_lam. wp_pures. wp_apply twp_ndnat; [done|].
-    iIntros (?) "_". by wp_apply twp_iter_inc.
+    iIntros (?) "#?". iIntros (?) "!> #? ?". wp_lam. wp_pures.
+    wp_apply twp_ndnat; [done|]. iIntros (?) "_". by wp_apply twp_siter.
   Qed.
 
-  (** [iter_inc_nd_forks] terminates *)
-  Lemma twp_iter_inc_nd_forks {N E d l} {c : nat} : ↑N ⊆ E →
-    [[{ mul_strmis N d l }]][nninv_wsats]
-      iter_inc_nd_forks #d #c #l @ E
+  (** [siter_nd_forks] terminates under [strmis] *)
+  Lemma twp_siter_nd_forks {N N' E Φ l} {f : val} {c : nat} :
+    (∀ l : loc,
+      [[{ nninvs 0 N (Φ l) }]][nninv_wsats] f #l [[{ RET #(); True }]]) -∗
+    [[{ strmis N N' Φ l }]][nninv_wsats]
+      siter_nd_forks f #c #l @ E
     [[{ RET #(); True }]].
   Proof.
-    iIntros (??) "#? Φ".
-    iInduction c as [|c] "IH"; wp_lam; wp_pures; [by iApply "Φ"|].
-    wp_apply twp_fork; [by wp_apply twp_iter_inc_nd|]. wp_pures.
+    iIntros "#?" (Ψ) "!> #? Ψ".
+    iInduction c as [|c] "IH"; wp_lam; wp_pures; [by iApply "Ψ"|].
+    wp_apply twp_fork; [by wp_apply twp_siter_nd|]. wp_pures.
     have ->: (S c - 1)%Z = c by lia. by iApply "IH".
   Qed.
 
-  (** [iter_inc_nd_forks_nd] terminates *)
-  Lemma twp_iter_inc_nd_forks_nd {N E d l} : ↑N ⊆ E →
-    [[{ mul_strmis N d l }]][nninv_wsats]
-      iter_inc_nd_forks_nd #d #l @ E
+  (** [siter_nd_forks_nd] terminates under [strmis] *)
+  Lemma twp_siter_nd_forks_nd {N N' E Φ l} {f : val} :
+    (∀ l : loc,
+      [[{ nninvs 0 N (Φ l) }]][nninv_wsats] f #l [[{ RET #(); True }]]) -∗
+    [[{ strmis N N' Φ l }]][nninv_wsats]
+      siter_nd_forks_nd f #l @ E
     [[{ RET #(); True }]].
   Proof.
-    iIntros (??) "#? ?". wp_lam. wp_pures. wp_apply twp_ndnat; [done|].
-    iIntros (?) "_". by wp_apply twp_iter_inc_nd_forks.
+    iIntros "#?" (?) "!> #? ?". wp_lam. wp_pures. wp_apply twp_ndnat; [done|].
+    iIntros (?) "_". by wp_apply twp_siter_nd_forks.
+  Qed.
+
+  (** [incr_faa] on [nninvs] over [has_mult] *)
+  Lemma twp_incr_faa {N E d l} : ↑N ⊆ E →
+    [[{ nninvs 0 N (has_mult d l) }]][nninv_wsats]
+      incr_faa d #l @ E
+    [[{ RET #(); True }]].
+  Proof.
+    iIntros (??) "#? Φ". wp_lam. wp_bind (FAA _ _).
+    iMod (nninvs_acc with "[//]") as "/= [[%k ↦] cl]"; [done|]. wp_faa.
+    iModIntro. iMod ("cl" with "[↦]") as "_".
+    { iExists _. by have ->: (k * d + d = (k + 1) * d)%Z by lia. }
+    iModIntro. wp_pures. by iApply "Φ".
+  Qed.
+
+  (** [may_incr_cas] on [nninvs] over [has_mult] *)
+  Lemma twp_may_incr_cas' {N E d l} {c : nat} : ↑N ⊆ E → d ≠ 0 →
+    [[{ nninvs 0 N (has_mult d l) }]][nninv_wsats]
+      may_incr_cas' d #c #l @ E
+    [[{ RET #(); True }]].
+  Proof.
+    iIntros (???) "#? Φ".
+    iInduction c as [|c] "IH"; wp_lam; wp_pures; [by iApply "Φ"|].
+    wp_bind (! _)%E. iMod (nninvs_acc with "[//]") as "/= [[%k ↦] cl]"; [done|].
+    wp_load. iModIntro. iMod ("cl" with "[↦]") as "_"; [by iExists _|].
+    iModIntro. wp_pures. wp_bind (CmpXchg _ _ _).
+    iMod (nninvs_acc with "[//]") as "/= [[%k' ↦] cl]"; [done|].
+    case (decide (k' = k))=> [->|neq].
+    - wp_apply (twp_cmpxchg_suc with "↦")=>//; [solve_vals_compare_safe|].
+      iIntros "↦". iMod ("cl" with "[↦]") as "_".
+      { iExists _. by have ->: (k * d + d = (k + 1) * d)%Z by lia. }
+      iModIntro. wp_pures. by iApply "Φ".
+    - wp_apply (twp_cmpxchg_fail with "↦")=>//.
+      { move=> [/Z.mul_reg_r]. lia. } { solve_vals_compare_safe. }
+      iIntros "↦". iMod ("cl" with "[↦]") as "_"; [by iExists _|]. iModIntro.
+      wp_pures. have ->: (S c - 1)%Z = c by lia. by iApply "IH".
+  Qed.
+  Lemma twp_may_incr_cas {N E d l} : ↑N ⊆ E → d ≠ 0 →
+    [[{ nninvs 0 N (has_mult d l) }]][nninv_wsats]
+      may_incr_cas d #l @ E
+    [[{ RET #(); True }]].
+  Proof.
+    iIntros (???) "#? Φ". wp_lam. wp_apply twp_ndnat; [done|].
+    iIntros (?) "_". by wp_apply twp_may_incr_cas'.
   Qed.
 End verify.
