nola/examples/logic/verify/strm_base.v
@@ -1,0 +1,20 @@
+(** * Base definitions for shared mutable singly linked streams *)
+
+From nola.examples.heap_lang Require Export notation.
+
+(** Calls [f] on the first [c] elements of the stream by [d] *)
+Definition siter : val :=
+  rec: "self" "f" "c" "l" :=
+    if: "c" = #0 then #() else "f" "l";; "self" "f" ("c" - #1) (! ("l" +ₗ #1)).
+
+(** Calls [iter] with a non-deterministic [c] *)
+Definition siter_nd : val := λ: "f" "l", siter "f" Ndnat "l".
+
+(** Forks [c] threads executing [siter_nd] *)
+Definition siter_nd_forks : val :=
+  rec: "self" "f" "c" "l" :=
+    if: "c" = #0 then #() else
+      Fork (siter_nd "f" "l");; "self" "f" ("c" - #1) "l".
+
+(** Calls [siter_nd_forks] with a non-deterministic [c] *)
+Definition siter_nd_forks_nd : val := λ: "f" "l", siter_nd_forks "f" Ndnat "l".
